Improve treatment of stub names
Removes some of the magic numbers in the backend, by defining constants
for the locations and numbers of stub functions. The stub numbering from BVL
onwards is done bottom-up, building on stack_to_lab. The stub numbering
down to BVL is top-down, i.e., clos_to_bvl allocates locations from 0.
Thus, only bvl_to_bvi is required to shift locations during compilation.

Closes #119

compiler/backend/bvl_to_bviScript.sml
@@ -1,5 +1,5 @@
 open preamble bvlTheory bviTheory;
-local open bvl_inlineTheory bvl_constTheory bvl_handleTheory bvi_letTheory in end;
+local open bvl_inlineTheory bvl_constTheory bvl_handleTheory bvi_letTheory bvpTheory in end;
 
 val _ = new_theory "bvl_to_bvi";
 
@@ -54,13 +54,18 @@ val alloc_glob_count_def = tDefine "alloc_glob_count" `
   (WF_REL_TAC `measure exp1_size`)
 
 val AllocGlobal_location_def = Define`
-  AllocGlobal_location = 100:num`;
+  AllocGlobal_location = bvp$num_stubs`;
 val CopyGlobals_location_def = Define`
-  CopyGlobals_location = 101:num`;
+  CopyGlobals_location = AllocGlobal_location+1`;
 val InitGlobals_location_def = Define`
-  InitGlobals_location = 102:num`;
-val num_stubs_def = Define`
-  num_stubs = 103:num`;
+  InitGlobals_location = CopyGlobals_location+1`;
+
+val AllocGlobal_location_eq = save_thm("AllocGlobal_location_eq",
+  ``AllocGlobal_location`` |> EVAL);
+val CopyGlobals_location_eq = save_thm("CopyGlobals_location_eq",
+  ``CopyGlobals_location`` |> EVAL);
+val InitGlobals_location_eq = save_thm("InitGlobals_location_eq",
+  ``InitGlobals_location`` |> EVAL);
 
 val AllocGlobal_code_def = Define`
   AllocGlobal_code = (0:num,
@@ -86,10 +91,13 @@ val InitGlobals_code_def = Define`
                    [Op (Const 1) []])]]
      (Call 0 (SOME start) [] (SOME (Var 0))))`;
 
-val bvi_stubs_def = Define `
-  bvi_stubs start n = [(AllocGlobal_location, AllocGlobal_code);
-                       (CopyGlobals_location, CopyGlobals_code);
-                       (InitGlobals_location, InitGlobals_code start n)]`;
+val stubs_def = Define `
+  stubs start n = [(AllocGlobal_location, AllocGlobal_code);
+                   (CopyGlobals_location, CopyGlobals_code);
+                   (InitGlobals_location, InitGlobals_code start n)]`;
+
+val num_stubs_def = Define`
+  num_stubs = bvp$num_stubs + 3`;
 
 val compile_op_def = Define `
   compile_op op c1 =
@@ -183,7 +191,7 @@ val compile_prog_def = Define `
   compile_prog start n prog =
     let k = alloc_glob_count (MAP (\(_,_,p). p) prog) in
     let (code,n1) = compile_list n prog in
-      (InitGlobals_location, bvi_stubs (num_stubs + 2 * start) k ++ code, n1)`;
+      (InitGlobals_location, bvl_to_bvi$stubs (num_stubs + 2 * start) k ++ code, n1)`;
 
 val optimise_def = Define `
   optimise =
